project part 3 complete

strings2.dfy
@@ -1,55 +1,53 @@
 predicate isPrefixPred(pre:string, str:string)
 {
-	(|pre| <= |str|) && pre == str[..|pre|]
+    (|pre| <= |str|) && (pre == str[..|pre|])
 }
 
 predicate isNotPrefixPred(pre:string, str:string)
 {
-    (|pre| > |str|) || pre != str[..|pre|] // not (isPrefixPred) and De Morgan
+    (|pre| > |str|) || (pre != str[..|pre|])
 }
 
 // Sanity check: Dafny should be able to automatically prove the following lemma
 lemma PrefixNegationLemma(pre:string, str:string)
-	ensures  isPrefixPred(pre,str) <==> !isNotPrefixPred(pre,str)
-	ensures !isPrefixPred(pre,str) <==>  isNotPrefixPred(pre,str)
+    ensures isPrefixPred(pre,str) <==> !isNotPrefixPred(pre,str)
+    ensures !isPrefixPred(pre,str) <==>  isNotPrefixPred(pre,str)
 {}
-
 
 predicate isSubstringPred(sub:string, str:string)
 {
-    (exists i :: ((0 <= i < |str|) && isPrefixPred(sub, str[i..])))
+    (exists i :: ((0 <= i < |str|) && (isPrefixPred(sub, str[i..])))) || (|sub| == 0)
 }
 
 predicate isNotSubstringPred(sub:string, str:string)
 {
-    forall i :: ((0 <= i < |str|) ==> (isNotPrefixPred(sub, str[i..])))
+    (forall i :: ((0 <= i < |str|) ==> (isNotPrefixPred(sub, str[i..])))) && (|sub| != 0)
 }
 
 // Sanity check: Dafny should be able to automatically prove the following lemma
 lemma SubstringNegationLemma(sub:string, str:string)
-	ensures  isSubstringPred(sub,str) <==> !isNotSubstringPred(sub,str)
-	ensures !isSubstringPred(sub,str) <==>  isNotSubstringPred(sub,str)
+    ensures  isSubstringPred(sub,str) <==> !isNotSubstringPred(sub,str)
+    ensures !isSubstringPred(sub,str) <==>  isNotSubstringPred(sub,str)
 {}
 
-
 // The following predicate should be true if and only if str1 and str2
-//  have a common substring of length k. 
-// You can refer to the preceding predicates within the body of 
-// this predicate.
+// have a common substring of length k.
 predicate haveCommonKSubstringPred(k:nat, str1:string, str2:string)
 {
-    (k == 0) || ((k <= |str1| && k <= |str2| && (forall i :: (0 <= i < |str1|-k) ==> (forall j :: (0 <= j < |str2|-k) ==> (exists d :: ((k == d) && isSubstringPred(str1[i..(i+k)], str2[j..(j+k)])))))))
+    // _s start _e end
+    (exists i_s, i_e :: (((0 <= i_s < (|str1| - k)) && (i_e == (i_s + k))) && isSubstringPred(str1[i_s..i_e], str2))) &&
+    (exists j_s, j_e :: (((0 <= j_s < (|str2| - k)) && (j_e == (j_s + k))) && isSubstringPred(str2[j_s..j_e], str1)))
 }
 
 predicate haveNotCommonKSubstringPred(k:nat, str1:string, str2:string)
 {
-	//TODO: your FOL formula should start with a forall
-    !haveCommonKSubstringPred(k, str1, str2)
-    //todo are we allowed to just negate the positive predicates?
+    // _s start _e end
+    (forall i_s, i_e :: (((0 <= i_s < (|str1| - k)) && (i_e == (i_s + k))) ==> isNotSubstringPred(str1[i_s..i_e], str2))) ||
+    (forall j_s, j_e :: (((0 <= j_s < (|str2| - k)) && (j_e == (j_s + k))) ==> isNotSubstringPred(str2[j_s..j_e], str1)))
 }
 
 // Sanity check: Dafny should be able to automatically prove the following lemma
 lemma commonKSubstringLemma(k:nat, str1:string, str2:string)
-	ensures  haveCommonKSubstringPred(k,str1,str2) <==> !haveNotCommonKSubstringPred(k,str1,str2)
-	ensures !haveCommonKSubstringPred(k,str1,str2) <==> haveNotCommonKSubstringPred(k,str1,str2)
+    ensures  haveCommonKSubstringPred(k,str1,str2) <==> !haveNotCommonKSubstringPred(k,str1,str2)
+    ensures !haveCommonKSubstringPred(k,str1,str2) <==> haveNotCommonKSubstringPred(k,str1,str2)
 {}
